Test/Concrete.v
@@ -3,81 +3,63 @@ Require Import SLFun.ConcreteProg.
 Definition f_aux  : fid := 0.
 Definition f_main : fid := 1.
 
-Definition s_aux : f_spec := {|
-  fs_arg_t := ptr;
-  fs_ret_t := nat;
-  fs_pre   := fun p m => Mem.read m p > 0;
-  fs_post  := fun p m0 r m1 => Mem.read m1 p = S r;
-|}.
-
-Definition s_main : f_spec := {|
-  fs_arg_t := unit;
-  fs_ret_t := unit;
-  fs_pre   := fun _ _ => True;
-  fs_post  := fun _ _ _ _ => True;
-|}.
-
-Inductive Sctx : scontext :=
-  | Sctx_aux  : Sctx f_aux  s_aux
-  | Sctx_main : Sctx f_main s_main.
-
-Definition i_aux : f_impl := {|
-  f_arg_t := ptr;
-  f_ret_t := nat;
-  f_body  := fun p =>
-    Bind (Read p) (fun x => Ret (pred x))
-|}.
+Definition SIG : sig_context :=
+  fun f => match f with
+  | 0 => Some (mk_f_sig ptr nat)
+  | 1 => Some (mk_f_sig unit unit)
+  | _ => None
+  end.
 
 Definition ptr0 : ptr := 42.
 Global Opaque ptr0.
 
-Definition i_main : f_impl := {|
-  f_arg_t := unit;
-  f_ret_t := unit;
-  f_body  := fun _ =>
-    Bind (Write ptr0 3) (fun _ =>
-    Bind (Call nat f_aux ptr0) (fun r =>
-          Assert (fun m => Mem.read m ptr0 = S r)))
-|}.
-
-Definition Cctx : context :=
+Definition IMPL : impl_context SIG :=
   fun f => match f with
-  | 0 => Some i_aux
-  | 1 => Some i_main
-  | _ => None
+  | 0 =>
+      fun (p : ptr) =>
+      Bind (Read p) (fun x => Ret (pred x))
+  | 1 =>
+      fun (_ : unit) =>
+      Bind (Write ptr0 3) (fun _ =>
+      Bind (@Call SIG _ f_aux eq_refl ptr0) (fun r =>
+            Assert (fun m => Mem.read m ptr0 = S r)))
+  | _ => tt
   end.
 
-Lemma match_aux:
-  f_match_spec Sctx i_aux s_aux.
-Proof.
-  constructor; intros p m; simpl.
-  case (Mem.read m p); simpl; try reflexivity.
-  inversion 1.
-Qed.
-
-Lemma match_main:
-  f_match_spec Sctx i_main s_main.
-Proof.
-  constructor; intros _ m _; simpl.
-  do 3 esplit. constructor.
-  simpl.
-  split.
-    { unfold Mem.read, Mem.write; destruct Mem.ptr_eq.
-      repeat constructor. congruence. }
-  auto.
-Qed.
+Definition SPECS : spec_context SIG :=
+  fun f => match f with
+  | 0 =>
+    let sg := mk_f_sig ptr nat in
+    eq {|
+      f_pre  := fun (p : f_arg_t sg) m => Mem.read m p > 0;
+      f_post := fun p m0 r m1 => Mem.read m1 p = S r;
+    |}
+  | 1 => eq {|
+      f_pre  := fun _ _ => True;
+      f_post := fun _ _ _ _ => True;
+    |}
+  | _ => tt
+  end.
 
 Lemma match_context:
-  context_match_spec Cctx Sctx.
+  context_match_spec IMPL SPECS.
 Proof.
-  inversion 1; simpl; (do 2 esplit; [reflexivity|]).
-  apply match_aux.
-  apply match_main.
+  intros [|[|]]; simpl. 3:constructor.
+  all:intros ? <-; unfold f_match_spec; simpl.
+  - (* aux *)
+    intros p m.
+    case (Mem.read m p); simpl; try reflexivity.
+    inversion 1.
+  - (* main *)
+    intros _ m _.
+    do 3 esplit; simpl.
+    + unfold Mem.read, Mem.write; destruct Mem.ptr_eq. 2:congruence.
+      repeat constructor.
+    + auto.
 Qed.
 
 Lemma context_oracle_free:
-  context_oracle_free Cctx.
+  context_oracle_free IMPL.
 Proof.
-  intros [|[|]] fi; simpl; simplify_eq 1; intros <- ?;
-  repeat constructor.
+  intros [|[|]]; simpl; repeat constructor.
 Qed.
